metric2/Classification.v
@@ -31,14 +31,14 @@ Definition stableMetric (ms:MetricSpace) :=
  forall e (x y:ms), ~~(ball e x y) -> ball e x y.
 
 Lemma stableEq : forall (ms:MetricSpace) (stable:stableMetric ms) (x y:ms),
- ~~(ms_eq x y) -> ms_eq x y.
+ ~~(st_eq x y) -> st_eq x y.
 Proof.
 intros ms stable x y Hxy.
 apply ball_eq.
 intros e.
 apply stable.
 revert Hxy.
-cut (ms_eq x y -> ball (m:=ms) e x y).
+cut (st_eq x y -> ball (m:=ms) e x y).
  tauto.
 intros H.
 rewrite H.
