model/metric2/CRmetric.v
@@ -40,11 +40,11 @@ Bind Scope CR_scope with CR.
 Definition inject_Q : Q -> CR := (@Cunit Q_as_MetricSpace).
 
 (* begin hide *)
-Add Morphism (inject_Q) with signature Qeq ==> (@ms_eq _) as inject_Q_wd.
+Add Morphism (inject_Q) with signature Qeq ==> (@st_eq _) as inject_Q_wd.
 exact (uc_wd (@Cunit Q_as_MetricSpace)).
 Qed.
 (* end hide *)
 
 Notation "' x" := (inject_Q x) : CR_scope.
 
-Notation "x == y" := (@ms_eq CR x y) (at level 70, no associativity) : CR_scope.
+Notation "x == y" := (@st_eq CR x y) (at level 70, no associativity) : CR_scope.
